\documentclass[12pt]{article}
\usepackage[left=0.5in, right=0.5in, top=0.5in, bottom=0.5in]{geometry}
\usepackage{ulem}
\usepackage{amsmath}
\usepackage{enumerate}

\begin{document}
\begin{flushleft}
Andy Liang

CSE 150 - Foundations of Computer Science: Honors

Professor Bender
\end{flushleft}
\medskip
\centerline{\uline{Homework 1A}}
\bigskip\bigskip

\noindent
\uline{Problem 1}
\\*\textbf{Write P$\implies$Q using $\land$ and $\neg$. Show that your two representation are equivalent.}
\medskip
\\*\uline{Response}
\\*P$\implies Q\iff \neg (P \land \neg Q)$
\bigskip
\\*
\begin{tabular}{c|c|c}
P & Q & $P \implies Q$\\
\hline
T & T & \textbf{T}\\
T & F & \textbf{F}\\
F & T & \textbf{T}\\
F & F & \textbf{T}\\
\end{tabular} 
\qquad\qquad
\begin{tabular}{c|c|c|c|c}
P & Q & $P \land Q$ &$P \land \neg Q$ & $\neg (P \land \neg Q)$\\
\hline
T & T & T & F & \textbf{T}\\
T & F & F & T & \textbf{F}\\
F & T & F & F & \textbf{T}\\
F & F & F & F & \textbf{T}\\

\end{tabular}
\bigskip\bigskip

\noindent
\uline{Problem 2}
\\*\textbf{Prove that the prepositional formulas}
\smallskip
\\*\centerline{\textbf{P $\lor$ Q $\lor$ R}}
\smallskip
\\*\textbf{and}
\smallskip
\\*\centerline{\textbf{(P $\land \neg$Q) $\lor$ (Q $\land \neg$R) $\lor$ (R $\land \neg$P) $\lor$ (P $\land$ Q $\land$ R)}}
\smallskip
\\*\textbf{are equivalent.}
\bigskip
\\*\uline{Response}
\bigskip
\\*
\begin{tabular}{c|c|c|c}
P & Q & R & $P \lor Q \lor R$\\
\hline
T & T & T & \textbf{T} \\
T & T & F & \textbf{T}\\
T & F & T & \textbf{T}\\
T & F & F & \textbf{T}\\
F & T & T & \textbf{T}\\
F & T & F & \textbf{T}\\
F & F & T & \textbf{T}\\
F & F & F & \textbf{F}\\
\end{tabular}
\qquad\qquad
\vspace{.5cm}
\\*\begin{tabular}{c|c|c|c|c|c|c|c}
P & Q & R & $P \land \neg Q$ & $Q \land \neg R$ & $R \land \neg P$ & $P \land Q \land R$ & (P $\land \neg$Q) $\lor$ (Q $\land \neg$R) $\lor$ (R $\land \neg$P) $\lor$ (P $\land$ Q $\land$ R)\\
\hline
T & T & T & F & F & F & T & \textbf{T}\\
T & T & F & F & T & F & F & \textbf{T}\\
T & F & T & T & F & F & F & \textbf{T}\\
T & F & F & T & F & F & F & \textbf{T}\\
F & T & T & F & F & T & F & \textbf{T}\\
F & T & F & F & T & F & F & \textbf{T}\\
F & F & T & F & F & T & F & \textbf{T}\\
F & F & F & F & F & F & F & \textbf{F}\\

\end{tabular}
\bigskip\bigskip
\noindent
\newpage\uline{Problem 3}
\begin{enumerate}[(a)]
\item \textbf{Write the biconditional ($\iff$) using only implies ($\implies$) and and ($\land$). Prove that the new version is equivalent.}
\item \textbf{Write it using only $\lor$ and $\neg$. Show your derivation.}
\end{enumerate}
\medskip
\uline{Response}
\begin{enumerate}[(a)]
\item $(P \iff Q) \iff ((P \implies Q) \land (Q \implies P))$
\vspace{0.25in}
\\*\begin{tabular}{c|c|c}
P & Q & $P \iff Q$\\
\hline
T & T & \textbf{T}\\
T & F & \textbf{F}\\
F & T & \textbf{F}\\
F & F & \textbf{T}\\
\end{tabular}
\qquad
\begin{tabular}{c|c|c|c|c}
P & Q & $P \implies Q$ & $Q \implies P$ & $(P \implies Q) \land (Q \implies P)$\\
\hline
T & T & T & T & \textbf{T}\\
T & F & F & T & \textbf{F}\\
F & T & T & F & \textbf{F}\\
F & F & T & T & \textbf{T}\\
\end{tabular}
\smallskip
\item $(P \iff Q) \iff \neg (\neg(\neg P \lor Q) \lor \neg(\neg Q \lor P)$
\vspace{0.25in}
\\* Proven Equivalence in Class:
\\*\centerline{$(P \implies Q) \iff (\neg P \lor Q)$ \hspace{0.25in} \& \hspace{0.25in} $(Q \implies P) \iff (\neg Q \lor P)$}
\medskip
\\*From 3a: 
\\*\centerline{$(P \iff Q) \iff ((P \implies Q) \land (Q \implies P))$}
\medskip
\\*Using DeMorgan's Law: 
\\*\centerline{$((P \implies Q) \land (Q \implies P)) \iff \neg (\neg(\neg P \lor Q) \lor \neg(\neg Q \lor P))$}
\vspace{0.25in}
\\*\begin{tabular}{c|c|c|c|c|c|c}
P & Q & 
$\neg P \lor Q$ & 
$\neg Q \lor P$ & 
$\neg (\neg P \lor Q)$ & 
$\neg (\neg Q \lor P)$ & 
$\neg (\neg P \lor Q) \lor \neg (\neg Q \lor P)$\\ 
%& $\neg (\neg(\neg P \lor Q) \lor \neg(\neg Q \lor P))$\\
\hline
T & T & T & T & F & F & F \\
T & F & F & T & T & F & T\\
F & T & T & F & F & T & T\\
F & F & T & T & F & F & F\\
\end{tabular}
\vspace{.25in}
\\*\begin{tabular}{c}
$\neg (\neg(\neg P \lor Q) \lor \neg(\neg Q \lor P))$\\
\hline
\textbf{T}\\
\textbf{F}\\
\textbf{F}\\
\textbf{T}\\
\end{tabular}
\end{enumerate}

\end{document}